an experiment with a different structure on function pointers

theories/lang/cpp/logic/heap_pred.v
@@ -547,17 +547,21 @@ Section with_cpp.
   (* this is the core definition that everything will be based on.
      it is really an assertion about assembly
    *)
-  Definition cptr_def {resolve : genv} (fs : function_spec) : Rep :=
+  Definition fptr_def {resolve : genv} (ft : type) (fs : function_spec) : Rep :=
     as_Rep (fun p =>
-         Forall (ti : thread_info), □ (Forall vs Q,
-         [| List.length vs = List.length fs.(fs_arguments) |] -*
-         fs.(fs_spec) ti vs Q -* fspec resolve.(genv_tu).(globals) (type_of_spec fs) ti (Vptr p) vs Q))%I.
-  Definition cptr_aux : seal (@cptr_def). by eexists. Qed.
-  Definition cptr := cptr_aux.(unseal).
-  Definition cptr_eq : @cptr = _ := cptr_aux.(seal_eq).
+              match ft with
+              | Tfunction cc ret args =>
+                Forall (ti : thread_info), □ (Forall vs Q,
+                [| List.Forall2 has_type vs args |] -*
+                fs.(fs_spec) ti vs Q -* fspec resolve.(genv_tu).(globals) ft ti (Vptr p) vs (fun r => [| has_type r ret |] ** Q r))
+              | _ => False
+              end)%I.
+  Definition fptr_aux : seal (@fptr_def). by eexists. Qed.
+  Definition fptr := fptr_aux.(unseal).
+  Definition fptr_eq : @fptr = _ := fptr_aux.(seal_eq).
 
-  Global Instance cptr_persistent {resolve} : Persistent (cptr resolve s).
-  Proof. rewrite cptr_eq. apply _. Qed.
+  Global Instance fptr_persistent {resolve ft} : Persistent (fptr resolve ft s).
+  Proof. rewrite fptr_eq /fptr_def; destruct ft; apply _. Qed.
 
   (** object identity *)
   Definition _identity (σ : genv) (cls : globname) (mdc : option globname)
@@ -611,8 +615,8 @@ Arguments primR {_ Σ resolve} ty q v : rename.
 Arguments refR {_ Σ} ty v : rename.
 
 
-Instance Persistent_spec `{Σ:cpp_logic ti} {resolve:genv} nm s :
-  Persistent (_at (Σ:=Σ) (_global (resolve:=resolve) nm) (cptr resolve s)) := _.
+Instance Persistent_spec `{Σ:cpp_logic ti} {resolve:genv} ft nm s :
+  Persistent (_at (Σ:=Σ) (_global (resolve:=resolve) nm) (fptr resolve ft s)) := _.
 
 #[deprecated(since="20200728", note="Use the constructor tactic instead")]
 Notation Rep_lequiv := Rep_ext (only parsing).
